

# Sets Cheatsheet

## Contents

<b>1</b>	<b>Geometric Series</b>	<b>2</b>
1.1	Examples . . . . .	2
<b>2</b>	<b>General Power Series</b>	<b>3</b>
2.1	Derivation . . . . .	3
2.2	Examples . . . . .	4
2.3	Error Checking . . . . .	4
2.4	Lagrange Error Checking . . . . .	5
2.4.1	Full Example . . . . .	5
2.4.2	Another Problem . . . . .	5

# 1 Geometric Series

Geometric Series are a special type of Power Series that can be rewritten in the form

$$f(x) = \frac{a_1}{1-r} = \sum_{n=0}^{\infty} a_1 * r^n$$

To find the interval of convergence, just remember that  $|r| < 1$

## 1.1 Examples

$$\begin{aligned} f(x) = \frac{1}{2-x}, c=0 &\Rightarrow f(x) = \frac{1}{2} * \frac{1}{1-\frac{x}{2}} \Rightarrow f(x) = \sum_{n=0}^{\infty} \frac{1}{2} * \left(\frac{x}{2}\right)^n \\ &\Rightarrow f(x) = \sum_{n=0}^{\infty} \left(\frac{1}{2}\right)^{n+1} x^n \end{aligned}$$

$$|r| < 1 \Rightarrow \left|\frac{x}{2}\right| < 1 \Rightarrow |x| < 2 \Rightarrow x \in (-2, 2)$$

If we change the center:

$$\begin{aligned} f(x) = \frac{1}{2-x}, c=5 &\Rightarrow f(x) = \frac{1}{2-5-(x-5)} \Rightarrow \frac{1}{-3-(x-5)} \\ &\Rightarrow -\frac{1}{3} * \frac{1}{1-\frac{-(x-5)}{3}} \Rightarrow \sum_{n=0}^{\infty} -\frac{1}{3} * \left(\frac{-(x-5)}{3}\right)^n \\ &\Rightarrow \sum_{n=0}^{\infty} \left(-\frac{1}{3}\right)^{n+1} (-(x-5))^n \end{aligned}$$

$$|r| < 1 \Rightarrow r \in (-1, 1) \Rightarrow \frac{-x+5}{3} \in (-1, 1) \Rightarrow -(x-5) \in (-3, 3) \Rightarrow x \in (2, 8)$$

Now let's completely change it up.

$$f(x) = \frac{3}{2x-1}, c=0 \Rightarrow f(x) = -3 * \frac{1}{1-2x} \Rightarrow * \sum_{n=0}^{\infty} -3 * (2x)^n, c \in \left(-\frac{1}{2}, \frac{1}{2}\right)$$

Let's move the center

$$\begin{aligned} f(x) = \frac{3}{2x-1}, c=-3 &\Rightarrow f(x) = \frac{1}{2(x+3)-5-6} \Rightarrow f(x) = -\frac{1}{11} * \frac{1}{1-\frac{2}{11}(x+3)} \\ &\Rightarrow f(x) = \sum_{n=0}^{\infty} -\frac{1}{11} * \left(\frac{2}{11}(x+3)\right)^n \\ \frac{2}{11}(x+3) \in (-1, 1) &\Rightarrow (x+3) \in \left(-\frac{11}{2}, \frac{11}{2}\right) \Rightarrow x \in \left(-\frac{17}{2}, \frac{5}{2}\right) \end{aligned}$$

What if there is no  $-x$ ? You can just do  $-(-x)$ . Remember: Basic Algebra will take you a long way.

$$f(x) = \frac{3}{x+2}, c=0 \implies f(x) = \frac{3}{2} * \frac{1}{1 - \frac{1}{2}(-x)}$$

What if your function looks a bit more complicated?

$$f(x) = \frac{4x-7}{2x^2+3x-2}, c=0 \implies f(x) = \frac{4x-7}{(2x-1)(x+2)} \implies f(x) = \frac{A}{2x-1} + \frac{B}{x+2}$$

$$A(x+2) + B(2x-1) = 4x-7 \implies Ax + 2Bx = 4x, 2A - B = -7 \implies B = 2A + 7$$

$$\implies A + 4A + 14 = 4 \implies 5A = -10 \implies A = -2, B = 3$$

$$f(x) = \frac{-2}{2x-1} + \frac{3}{x+2}$$

Solve it normally from here.

## 2 General Power Series

$$f(x) = \sum_{n=0}^{\infty} \frac{f^{(n)}(c)}{n!} (x-c)^n$$

### 2.1 Derivation

We take general power series to be something like the following:

$$f(x) = 1 + x + 2x^2 + 3x^3 + \dots + nx^n + \dots$$

or

$$f(x) = 1 + x + \frac{1}{2}x^2 + \frac{1}{3}x^3 + \dots + \frac{1}{n}x^n + \dots$$

So generally:

$$f(x) = \sum_{n=0}^{\infty} a_n (x-c)^n$$

Instead of  $a_i$  because the coefficient changes for each element in the series. Let's expand this series:

$$f(x) = a_0 + c + a_1(x-c) + a_2(x-c)^2 + a_3(x-c)^3 + \dots + a_n(x-c)^n + \dots$$

Take its derivative:

$$f'(x) = 0 + a_1 + 2a_2(x-c) + 3a_3(x-c)^2 + \dots + na_n(x-c)^{n-1} + \dots$$

Notice how  $f'(0) = a_1$ .

$$f''(x) = 0 + 0 + 2a_2 + 6a_3(x-c) + \dots + n(n-1)a_n(x-c)^{n-2} + \dots$$

Notice how  $f''(0) = 2a_2$  and  $f'''(0) = 6a_3$ . In order to get the  $a_n$  term, you just need to take  $f^{(n)}(c)$  and divide it by  $n!$

Put it together, and you'll get the equation we started with.

## 2.2 Examples

$$\begin{aligned} f(x) = e^x, c = 0 &\implies f(x) = \sum_{n=0}^{\infty} \frac{e^0}{n!} (x)^n \implies f(x) = \sum_{n=0}^{\infty} \frac{x^n}{n!} \\ &\implies 1 + x + \frac{1}{2}x^2 + \frac{1}{3}x^3 + \dots + \frac{1}{n}x^n + \dots \end{aligned}$$

Evaluate a geometric series using Taylor series

$$\begin{aligned} f(x) = \frac{1}{1-2x}, c = 0 &\implies \frac{1}{\frac{1-2(0)}{0!}} + \frac{\frac{2}{(1-2c)^2}}{1!}x + \frac{\frac{8}{(1-2c)^3}}{2!}x + \frac{\frac{48}{(1-2c)^4}}{3!}x + \dots \\ &\implies 1 + \frac{2}{(1-2c)^2}x + \frac{4}{(1-2c)^3}x^2 + \frac{8}{(1-2c)^4}x^3 + \dots \end{aligned}$$

General term:  $2^n x^n$ .

We would have gotten the same thing if we used the power series expansion of the Taylor series expansion. As with most things in algebra, pick the method that's **most convenient for you**.

## 2.3 Error Checking

In an ideal world, you want to know how far off your estimates are. For alternating series, this process is pretty easy.

$$f(x) = 1 - x + \frac{x}{2!} - \frac{x}{3!} + \frac{x}{4!} - \frac{x}{5!} + \frac{x}{6!} - \frac{1}{7!} + \dots + \frac{1}{n!}(-1)^n + \dots$$

Let's choose the first four terms for our **Taylor Polynomial**, which will be represented by  $P_n(x)$  where  $n$  is the degree.

$$P_4(x) = 1 - x + \frac{1}{2}x^2 - \frac{1}{3}x^3$$

Let's set the remainder terms to  $R_5(x)$ . We can call the error  $E(x)$ .

$$E(x) = |P_4(x) - R_5(x)|$$

Since you will never truly know  $R_5(x)$  or any  $R_n(x)$  for that matter, you will never know the true error. But you can set an upper bound on that error, which is pretty easy in alternating power series.

$$E(x) \leq P_{n+1}(x) - P_n(x)$$

A fancy way of saying, the term right after is the highest the error can be. It's because you will never add back what you subtracted, always less.

## 2.4 Lagrange Error Checking

If your series **isn't alternating**, you can use Lagrange Error Checking. Although the proof is complicated, it's pretty simple

$$E(x) \leq \left| \frac{\max_{z \in [x, c]} f^{(n+1)}(z)}{(n+1)!} \right| (x - c)^{n+1}$$

The proof isn't necessary for Calc BC. You can find it online.

### 2.4.1 Full Example

Find the first four terms about  $c = 2$  for  $\ln|x + 1|$ .

We can start with its derivative,  $\frac{1}{x+1}$ .

For simplicity, we will use a geometric series. Say we wanted to find  $\ln|\frac{3}{2}|$  and approximate error to be 0.05 or less

$$\begin{aligned} \frac{1}{x-1} &= \frac{1}{1-(x-2)+2} = \frac{1}{-1-(x-2)} = -\frac{1}{1-(-(x-2))} \\ \Rightarrow \sum_{n=0}^{\infty} -(-(x-2))^n &= \sum_{n=0}^{\infty} (-1)^{n+1}(x-2)^n = -1 + (x-2) - \frac{1}{2}(x-2)^2 + \frac{1}{3}(x-2)^3 + \dots \\ \int -\frac{1}{1-(-(x-2))} dx &= \int -1 + (x-2) - \frac{1}{2}(x-2)^2 + \frac{1}{3}(x-2)^3 + \dots dx \\ \Rightarrow -\ln|1-(-(x-2))| &= C - x + \frac{(x-2)^2}{2} - \frac{(x-2)^3}{3 * 2!} + \frac{(x-2)^4}{4 * 3!} + \dots \\ &\rightarrow \ln|1-(-(2-2))| = \ln|1| \\ &\rightarrow C + x - \frac{(x-2)^2}{2} + \frac{(x-2)^3}{3 * 2!} - \frac{(x-2)^4}{4 * 3!} + \dots \\ &\rightarrow \ln|1| = C + 2 + 0 + \dots \rightarrow C = -2 \\ \Rightarrow \ln|1-(-(x-2))| &= -2 + x - \frac{(x-2)^2}{2} + \frac{(x-2)^3}{3 * 2!} - \frac{(x-2)^4}{4 * 3!} + \dots \\ \Rightarrow \ln|\frac{3}{2}| = \ln|1-(-(\frac{5}{2}-2))| &= (\frac{5}{2}-2) - \frac{(\frac{5}{2}-2)^2}{2} + \frac{(\frac{5}{2}-2)^3}{3 * 2!} - \frac{(\frac{5}{2}-2)^4}{4 * 3!} + \dots \\ &\Rightarrow \frac{1}{2} - \frac{1}{2} * (\frac{1}{2})^2 + \frac{1}{3} * (\frac{1}{2})^3 - \frac{1}{4} * (\frac{1}{2})^4 + \dots \end{aligned}$$

Since it's an alternating series, it should be pretty simple to solve for from here.

### 2.4.2 Another Problem

$$\sin(5x + \frac{\pi}{4}) = \sin(5(x + \frac{\pi}{20}))$$